Use app_list for longer in bvl_to_bvi
Push bad appends up to the top level, so they only happen once.
See #133.

compiler/backend/bvl_to_bviScript.sml
@@ -133,6 +133,10 @@ val compile_op_def = Define `
 
 val _ = temp_overload_on("++",``SmartAppend``);
 
+val compile_aux_def = Define`
+  compile_aux (k,args,p) =
+    List[(num_stubs + 2 * k + 1, args, bvi_let$compile_exp p)]`;
+
 val compile_exps_def = tDefine "compile_exps" `
   (compile_exps n [] = ([],Nil,n)) /\
   (compile_exps n ((x:bvl$exp)::y::xs) =
@@ -152,7 +156,7 @@ val compile_exps_def = tDefine "compile_exps" `
        let (c2,aux2,n2) = compile_exps n1 [x0] in
        let n3 = n2 + 1 in
          ([Call 0 (SOME (num_stubs + 2 * n2 + 1)) c1 NONE],
-          aux1++aux2++List[(n2,LENGTH args,HD c2)], n3)
+          aux1++aux2++compile_aux(n2,LENGTH args,HD c2), n3)
      else
        let (c1,aux1,n1) = compile_exps n xs in
        let (c2,aux2,n2) = compile_exps n1 [x2] in
@@ -171,7 +175,7 @@ val compile_exps_def = tDefine "compile_exps" `
      let (c1,aux1,n1) = compile_exps n args in
      let (c2,aux2,n2) = compile_exps n1 [x0] in
      let (c3,aux3,n3) = compile_exps n2 [x2] in
-     let aux4 = List[(n3,LENGTH args,HD c2)] in
+     let aux4 = compile_aux(n3,LENGTH args,HD c2) in
      let n4 = n3 + 1 in
        ([Call 0 (SOME (num_stubs + 2 * n3 + 1)) c1 (SOME (HD c3))],
         aux1++aux2++aux3++aux4, n4)) /\
@@ -207,12 +211,10 @@ val compile_exps_SING = store_thm("compile_exps_SING",
 val compile_single_def = Define `
   compile_single n (name,arg_count,exp) =
     let (c,aux,n1) = compile_exps n [exp] in
-      (MAP (\(k,args,p).
-          (num_stubs + 2 * k + 1,args,bvi_let$compile_exp p)) (append aux) ++
-       [(num_stubs + 2 * name,arg_count,HD c)],n1)`
+      (aux ++ List [(num_stubs + 2 * name,arg_count,HD c)],n1)`
 
 val compile_list_def = Define `
-  (compile_list n [] = ([],n)) /\
+  (compile_list n [] = (List [],n)) /\
   (compile_list n (p::progs) =
      let (code1,n1) = compile_single n p in
      let (code2,n2) = compile_list n1 progs in
@@ -222,7 +224,7 @@ val compile_prog_def = Define `
   compile_prog start n prog =
     let k = alloc_glob_count (MAP (\(_,_,p). p) prog) in
     let (code,n1) = compile_list n prog in
-      (InitGlobals_location, bvl_to_bvi$stubs (num_stubs + 2 * start) k ++ code, n1)`;
+      (InitGlobals_location, bvl_to_bvi$stubs (num_stubs + 2 * start) k ++ append code, n1)`;
 
 val optimise_def = Define `
   optimise cut_size ls =
