compiler/eval/compilerComputeLib.sml
@@ -304,6 +304,7 @@ val add_compiler_compset = computeLib.extend_compset
     ,bvl_to_bviTheory.ListLength_location_eq
     ,bvl_to_bviTheory.compile_int_def
     ,bvl_to_bviTheory.compile_exps_def
+    ,bvl_to_bviTheory.compile_aux_def
     ,bvl_to_bviTheory.optimise_def
     ,bvl_to_bviTheory.default_config_def
       (* ---- bvi_let ---- *)
